json/Theorems/Parser.v
@@ -64,3 +64,44 @@ Proof.
       }
     + reflexivity.
 Qed.
+
+Theorem all_aux_saturation_aux : forall A I E processor,
+  (forall suffix response text,
+    processor text = Ok (response, suffix) ->
+    length suffix < length text) ->
+  forall n text fuel,
+  (S (length text)) < n ->
+  (S (length text)) <= fuel ->
+  @all_aux A I E processor (S (length text)) text = @all_aux A I E processor fuel text.
+Proof.
+  intros A I E processor processor_good.
+  induction n; intros text fuel.
+  - intros H. inversion H.
+  - intros text_bounded enough_fuel.
+    destruct text as [|text_head text_tail].
+    destruct fuel; try inversion enough_fuel. reflexivity. simpl. destruct (processor []) eqn:response_definition.
+    destruct x as [response suffix].
+    exfalso. assert (@length I suffix < @length I nil).
+    apply processor_good with (response := response) (suffix := suffix).
+    apply response_definition.
+    inversion H1.
+    reflexivity. simpl in text_bounded. 
+    destruct fuel. exfalso. inversion enough_fuel.
+    simpl. destruct (processor (text_head :: text_tail)) eqn:response_definition.
+    + destruct x as [val rest].
+      replace (all_aux processor fuel rest) with (all_aux processor (S (length text_tail)) rest).
+      reflexivity.
+      assert (length rest < length (text_head :: text_tail)). {
+        apply processor_good with (response := val).
+        apply response_definition.
+      } {
+      replace
+        (all_aux processor (S (length text_tail)) rest)
+      with
+        (all_aux processor (S (length rest)) rest).
+      apply IHn. simpl in H. lia. lia.
+      apply IHn. simpl in H. lia.
+      simpl in H. lia.
+      }
+    + reflexivity.
+Qed.
